theories/SimplyTypedLambdaCalculus/StrongNormalisation.v
@@ -1,44 +1,41 @@
-From FormArith.SimplyTypedLambdaCalculus Require Import Definitions.
-
-Require Import Relations.Relations.
+From FormArith.SimplyTypedLambdaCalculus Require Import Term Typing.
 
 
 Inductive SN: term -> Prop :=
   | Strong (t: term) :
       (forall (t': term), t ~> t' -> SN t') -> SN t.
 
-Locate "~>*".
-
 Fixpoint reducible (A: type) (t: term): Prop :=
   match A with
   | Base => SN t
   | Arr A B => forall (u: term), reducible A u -> reducible B (App t u)
-  | Prod A B => reducible A (Pr1 t) /\ reducible B (Pr2 t)
+  | Prod A B => reducible A (ProjL t) /\ reducible B (ProjR t)
   | Sum A B =>
       SN t /\
-      (forall u, t ~>* In1 u -> reducible A u) /\
-      (forall v, t ~>* In2 v -> reducible B v)
+      (forall u, t ~>* InjL u -> reducible A u) /\
+      (forall v, t ~>* InjR v -> reducible B v)
   end.
 
 Definition neutral (t: term): Prop :=
   match t with
-  | Lam _ | Pair _ _ | In1 _ | In2 _ => False
+  | Lam _ | Pair _ _ | InjL _ | InjR _ => False
   | _ => True
   end.
 
 Inductive sub_term: term -> term -> Prop :=
-  | Sub_app1 (t1 t2: term) : sub_term t1 (App t1 t2)
-  | Sub_app2 (t1 t2: term) : sub_term t2 (App t1 t2)
-  | Sub_lam (t: term) : sub_term t (Lam t)
-  | Sub_pair1 (t1 t2: term): sub_term t1 (Pair t1 t2)
-  | Sub_pair2 (t1 t2: term): sub_term t2 (Pair t1 t2)
-  | Sub_pr1 (t: term): sub_term t (Pr1 t)
-  | Sub_pr2 (t: term): sub_term t (Pr2 t)
-  | Sub_pat1 (t1 t2 t3: term): sub_term t1 (Pat t1 t2 t3)
-  | Sub_pat2 (t1 t2 t3: term): sub_term t2 (Pat t1 t2 t3)
-  | Sub_pat3 (t1 t2 t3: term): sub_term t3 (Pat t1 t2 t3)
-  | Sub_in1 (t: term): sub_term t (In1 t)
-  | Sub_in2 (t: term): sub_term t (In2 t).
+  | Sub_App1 (t1 t2: term) : sub_term t1 (App t1 t2)
+  | Sub_App2 (t1 t2: term) : sub_term t2 (App t1 t2)
+  | Sub_Lam (t: term) : sub_term t (Lam t)
+  | Sub_Pair1 (t1 t2: term): sub_term t1 (Pair t1 t2)
+  | Sub_Pair2 (t1 t2: term): sub_term t2 (Pair t1 t2)
+  | Sub_ProjL (t: term): sub_term t (ProjL t)
+  | Sub_ProjR (t: term): sub_term t (ProjR t)
+  | Sub_Case1 (t1 t2 t3: term): sub_term t1 (Case t1 t2 t3)
+  | Sub_Case2 (t1 t2 t3: term): sub_term t2 (Case t1 t2 t3)
+  | Sub_Case3 (t1 t2 t3: term): sub_term t3 (Case t1 t2 t3)
+  | Sub_InjL (t: term): sub_term t (InjL t)
+  | Sub_InjR (t: term): sub_term t (InjR t).
+
 
 Lemma SN_lam (t: term):
   SN t -> SN (Lam t).
@@ -47,7 +44,7 @@ Proof.
 
   apply SN_ind; intros ? _ H.
   apply Strong; intros ? Hbeta.
-  inversion Hbeta; subst.
+  inv Hbeta.
   now apply H.
 Qed.
 
@@ -66,53 +63,53 @@ Proof.
   (** Classical Lambda calculus *)
   - apply IH with (App u t2).
     + now apply Beta_AppL.
-    + apply Sub_app1.
+    + apply Sub_App1.
 
   - apply IH with (App t1 u).
     + now apply Beta_AppR.
-    + apply Sub_app2.
+    + apply Sub_App2.
 
   - apply IH with (Lam u).
     + now apply Beta_Lam.
-    + apply Sub_lam.
+    + apply Sub_Lam.
 
   (** Pairs and projections *)
   - apply IH with (Pair u t2).
     + now apply Beta_Pair1.
-    + apply Sub_pair1.
+    + apply Sub_Pair1.
 
   - apply IH with (Pair t1 u).
     + now apply Beta_Pair2.
-    + apply Sub_pair2.
+    + apply Sub_Pair2.
 
-  - apply IH with (Pr1 u).
-    + now apply Beta_Pr1.
-    + apply Sub_pr1.
+  - apply IH with (ProjL u).
+    + now apply Beta_ProjL.
+    + apply Sub_ProjL.
 
-  - apply IH with (Pr2 u).
-    + now apply Beta_Pr2.
-    + apply Sub_pr2.
+  - apply IH with (ProjR u).
+    + now apply Beta_ProjR.
+    + apply Sub_ProjR.
 
   (** Sum types *)
-  - apply IH with (Pat u t2 t3).
-    + now apply Beta_Pat1.
-    + apply Sub_pat1.
+  - apply IH with (Case u t2 t3).
+    + now apply Beta_Case1.
+    + apply Sub_Case1.
 
-  - apply IH with (Pat t1 u t3).
-    + now apply Beta_Pat2.
-    + apply Sub_pat2.
+  - apply IH with (Case t1 u t3).
+    + now apply Beta_Case2.
+    + apply Sub_Case2.
 
-  - apply IH with (Pat t1 t2 u).
-    + now apply Beta_Pat3.
-    + apply Sub_pat3.
+  - apply IH with (Case t1 t2 u).
+    + now apply Beta_Case3.
+    + apply Sub_Case3.
 
-  - apply IH with (In1 u).
-    + now apply Beta_In1.
-    + apply Sub_in1.
+  - apply IH with (InjL u).
+    + now apply Beta_InjL.
+    + apply Sub_InjL.
 
-  - apply IH with (In2 u).
-    + now apply Beta_In2.
-    + apply Sub_in2.
+  - apply IH with (InjR u).
+    + now apply Beta_InjR.
+    + apply Sub_InjR.
 Qed.
 
 Lemma SN_var_app (t: term) (n: var):
@@ -120,7 +117,7 @@ Lemma SN_var_app (t: term) (n: var):
 Proof.
   intros ?.
   apply (SN_sub_term (App t (Var n))); [ assumption |].
-  apply Sub_app1.
+  apply Sub_App1.
 Qed.
 
 Lemma SN_inverted (t: term):
@@ -137,23 +134,23 @@ Proof.
   induction A as [
     | A [IHA1 [IHA2 IHA3]] B [IHB1 [IHB2 IHB3]]
     | A [IHA1 [IHA2 IHA3]] B [IHB1 [IHB2 IHB3]]
-    | A [IHA1 [IHA2 IHA3]] B [IHB1 [IHB2 IHB3]]].
-  - do 3 split.
-    + intros.
-      apply SN_inverted with t'; [| assumption ].
-      now apply SN_inverted with t.
+    | A [IHA1 [IHA2 IHA3]] B [IHB1 [IHB2 IHB3]]
+  ].
 
-    + intros.
+  - split; [| split ]; simpl.
+    + now intros.
+
+    + intros t u ? ?.
+      apply Strong; intros.
       apply SN_inverted with u; [| assumption ].
       now apply SN_inverted with t.
 
-    + assumption.
+    + intros.
+      now apply Strong.
 
   - split; [| split ]; simpl.
     + intros ? Hred.
-      apply Strong.
-
-      intros ? ?.
+      apply Strong; intros.
       apply SN_inverted with t; [| assumption ].
       apply SN_var_app with 0.
 
@@ -164,14 +161,16 @@ Proof.
 
     + intros t ? IHred ? u Hred.
       apply IHB2 with (App t u).
-      * apply IHred, Hred.
+      * apply IHred.
+        apply Hred.
       * now apply Beta_AppL.
 
     + intros ? ? Hredt ? Hredu.
       apply IHA1 in Hredu as HSNu.
-      induction HSNu as [ u _ IHu ].
 
+      induction HSNu as [ u _ IHu ].
       apply IHB3; [ exact I |].
+
       inversion 1; subst.
       * contradiction.
       * now apply Hredt.
@@ -180,58 +179,61 @@ Proof.
 
   - split; [| split ]; simpl.
     + intros t [Hred _].
-      apply IHA1 in Hred. apply SN_sub_term with (t' := t) in Hred.
-      * assumption.
-      * apply Sub_pr1.
+      apply IHA1 in Hred.
+      apply SN_sub_term with (t' := t) in Hred; [ assumption |].
+      apply Sub_ProjL.
 
-    + intros t u [Hred1 Hred2] Hstep. split.
-      * apply (IHA2 (Pr1 t) _ Hred1). now apply Beta_Pr1.
-      * apply (IHB2 (Pr2 t) _ Hred2). now apply Beta_Pr2.
+    + intros t u [Hred1 Hred2] Hstep.
+      split.
+      * apply (IHA2 (ProjL t) _ Hred1).
+        now apply Beta_ProjL.
+      * apply (IHB2 (ProjR t) _ Hred2).
+        now apply Beta_ProjR.
 
-    + intros t Hneu H. split.
-      * apply IHA3; [ exact I | ]. intros t' Hstep. inv Hstep; [| destruct Hneu ].
-        apply (H s' H1).
-      * apply IHB3; [ exact I | ]. intros t' Hstep. inv Hstep; [| destruct Hneu ].
-        apply (H s' H1).
+    + intros t Hneu H.
+      split; [ apply IHA3 | apply IHB3 ]; simpl.
+      all: try exact I.
+      all: intros t' Hstep.
+      all: inv Hstep; [| destruct Hneu ].
+      all: apply (H s' H1).
 
-  - split; [| split]; simpl.
-    + intros t [HSN _]. apply HSN.
+  - split; [| split ]; simpl.
+    + intros t [HSN _].
+      apply HSN.
 
-    + intros t u [Hredt1 [Hredt2 Hredt3]] Hbeta. split; [| split].
-      * apply (SN_inverted t Hredt1). assumption.
-      * intros. apply Hredt2.
-        apply rt_trans with u; [| assumption ].
-        now apply rt_step.
-      * intros. apply Hredt3.
-        apply rt_trans with u; [| assumption ].
-        now apply rt_step.
+    + intros t u [Hredt1 [Hredt2 Hredt3]] Hbeta.
+      split.
+      { now apply (SN_inverted t Hredt1). }
 
-    + intros t Hneu H. split; [| split ].
-      * apply Strong. intros t' ?. apply H. assumption.
-      * intros u Hbeta. rewrite clos_rt_rt1n_iff in Hbeta.
-        inv Hbeta; [ destruct Hneu |].
-        apply H with y; [ assumption |]. apply clos_rt_rt1n_iff. assumption.
-      * intros u Hbeta. rewrite clos_rt_rt1n_iff in Hbeta.
-        inv Hbeta; [ destruct Hneu |].
-        apply H with y; [ assumption |]. apply clos_rt_rt1n_iff. assumption.
+      split; intros; [ apply Hredt2 | apply Hredt3 ].
+      all: apply rt_trans with u; [| assumption ].
+      all: now apply rt_step.
+
+    + intros t Hneu H.
+      split.
+      { apply Strong; intros. now apply H. }
+
+      split.
+      all: intros u Hbeta.
+      all: rewrite clos_rt_rt1n_iff in Hbeta.
+      all: inv Hbeta; [ destruct Hneu |].
+      all: apply H with y; [ assumption |].
+      all: now apply clos_rt_rt1n_iff.
 Qed.
 
 Lemma SN_subst (t: term) (σ: var -> term):
   SN t -> forall (u: term), t = u.[σ] -> SN u.
 Proof.
   induction 1 as [? _ IHt]; intros; subst.
-
-  apply Strong.
-  intros t ?.
-
+  apply Strong; intros t ?.
   apply IHt with t.[σ].
   - now apply beta_subst.
   - reflexivity.
 Qed.
 
 Lemma SN_ind_pair (P : term -> term -> Prop):
-  (forall t u, (forall t' u', ((t = t' /\ u ~> u') \/ (t ~> t' /\ u = u')) -> P t' u') -> P t u)
-    -> forall t u, SN t -> SN u -> P t u.
+  (forall t u, (forall t' u', ((t = t' /\ u ~> u') \/ (t ~> t' /\ u = u')) -> P t' u') -> P t u) ->
+    forall t u, SN t -> SN u -> P t u.
 Proof.
   intros IH ? ? Hsnt.
   revert u.
@@ -249,36 +251,43 @@ Proof.
 Qed.
 
 Lemma SN_triple_ind (P : term -> term -> term -> Prop):
-  (forall t u v, (forall t' u' v',
-                ((t = t' /\ u = u' /\ v ~> v') \/
-                   (t = t' /\ u ~> u' /\ v = v') \/
-                   (t ~> t' /\ u = u' /\ v = v'))
-                -> P t' u' v') -> P t u v)
-    -> forall t u v, SN t -> SN u -> SN v -> P t u v.
+  (forall t u v,
+    (forall t' u' v',
+      ((t = t' /\ u = u' /\ v ~> v') \/
+        (t = t' /\ u ~> u' /\ v = v') \/
+        (t ~> t' /\ u = u' /\ v = v')) -> P t' u' v') -> P t u v) ->
+  forall t u v, SN t -> SN u -> SN v -> P t u v.
 Proof.
   intros IH t u v Hsnt.
   revert u v.
 
   induction Hsnt as [? _ IHt].
-  intros u v Hsnu. revert v.
+  intros u v Hsnu.
+
+  revert v.
   induction Hsnu as [? HSNu IHu].
+
   intros v Hsnv.
   induction Hsnv as [? HSNv IHv].
   apply IH.
 
   intros ? ? ? [[? [? ?]] | [[? [? ?]] | [? [? ?]]]]; subst.
   - now apply IHv.
-  - apply IHu.
-    + assumption.
-    + apply Strong. intros. now apply HSNv.
-  - apply IHt.
-    + assumption.
-    + apply Strong. intros. now apply HSNu.
-    + apply Strong. intros. now apply HSNv.
+
+  - apply IHu; [ assumption |].
+    apply Strong; intros.
+    now apply HSNv.
+
+  - apply IHt; [ assumption | |].
+    + apply Strong; intros.
+      now apply HSNu.
+    + apply Strong; intros.
+      now apply HSNv.
 Qed.
 
 Lemma reducible_abs (v: term) (A B: type):
-  (forall (u: term), reducible A u -> reducible B v.[u/]) -> reducible (Arr A B) (Lam v).
+  (forall (u: term), reducible A u -> reducible B v.[u/]) ->
+    reducible (Arr A B) (Lam v).
 Proof.
   intros Hred u Hredu.
   specialize (reducible_is_SN A) as [HA1 [HA2 HA3]].
@@ -299,10 +308,10 @@ Proof.
   apply HB3; [ exact I |].
   intros t Hbeta.
 
-  inversion Hbeta; subst.
+  inv Hbeta.
   - now apply Hred.
 
-  - inversion H2; subst.
+  - inv H2.
     apply IH; [ .. | assumption ].
     { now right. }
 
@@ -317,14 +326,13 @@ Proof.
     + now apply HA2 with y.
 Qed.
 
-
 Lemma reducible_var (A: type) (x: var) (Γ: var -> type):
   Γ ⊢ Var x : A -> reducible A (Var x).
 Proof.
-  intros. specialize (reducible_is_SN A) as (_ & _ & HA3).
-  apply HA3.
-  - exact I.
-  - inversion 1.
+  intros.
+  specialize (reducible_is_SN A) as (_ & _ & HA3).
+  apply HA3; [ exact I |].
+  inversion 1.
 Qed.
 
 Lemma reducible_pair (A B: type) (u v: term):
@@ -332,141 +340,167 @@ Lemma reducible_pair (A B: type) (u v: term):
   reducible B v ->
   reducible (Prod A B) (Pair u v).
 Proof.
-  intros Hredu Hredv. simpl.
+  intros Hredu Hredv; simpl.
+
   specialize (reducible_is_SN A) as (HA1 & HA2 & HA3).
   specialize (reducible_is_SN B) as (HB1 & HB2 & HB3).
+
   assert (HSNu: SN u) by now apply HA1.
   assert (HSNv: SN v) by now apply HB1.
+
   revert Hredu Hredv.
-  apply SN_ind_pair with (t := u) (u := v); [| assumption | assumption ].
-  intros u' v' IH.
-  intros Hredu' Hredv'. split.
-  - apply HA3; [exact I |].
-    intros t' Hred. inv Hred.
-    + inv H0.
-      * apply IH.
-        -- now right.
-        -- now apply HA2 with u'.
-        -- assumption.
-      * apply IH.
-        -- now left.
-        -- assumption.
-        -- now apply HB2 with v'.
-    + assumption.
-  - apply HB3; [exact I |].
-    intros t' Hred. inv Hred.
-    + inv H0.
-      * apply IH.
-        -- now right.
-        -- now apply HA2 with u'.
-        -- assumption.
-      * apply IH.
-        -- now left.
-        -- assumption.
-        -- now apply HB2 with v'.
-    + assumption.
+  apply SN_ind_pair with (t := u) (u := v); [| assumption.. ].
+
+  intros u' v' IH Hredu' Hredv'.
+  split; [ apply HA3 | apply HB3 ]; simpl.
+  all: try exact I.
+  all: intros t' Hred.
+  all: inv Hred; [| assumption ].
+  all: inv H0.
+
+  - apply IH; [| | assumption ].
+    + now right.
+    + now apply HA2 with u'.
+
+  - apply IH; [| assumption |].
+    + now left.
+    + now apply HB2 with v'.
+
+  - apply IH; [| | assumption ].
+    + now right.
+    + now apply HA2 with u'.
+
+  - apply IH; [| assumption |].
+    + now left.
+    + now apply HB2 with v'.
 Qed.
 
-Lemma reducible_sum1 (A B: type) (s: term):
+Lemma reducible_sum_injL (A B: type) (s: term):
   reducible A s ->
-  reducible (Sum A B) (In1 s).
+  reducible (Sum A B) (InjL s).
 Proof.
-  intros Hreds. simpl.
+  intros Hreds; simpl.
+
   specialize (reducible_is_SN A) as (HA1 & HA2 & HA3).
   assert (HSN: SN s) by now apply HA1.
-  induction HSN as [s _ IH]. split.
-  - apply Strong. intros t' Hstep. inv Hstep. apply IH.
-    + assumption.
+
+  induction HSN as [s _ IH].
+  split.
+  { apply Strong; intros t' Hstep.
+    inv Hstep.
+    apply IH; [ assumption |].
+    now apply HA2 with s. }
+
+  all: split.
+  all: intros ? Hbeta.
+  all: rewrite clos_rt_rt1n_iff in Hbeta.
+  all: inv Hbeta; try assumption.
+  all: inv H.
+
+  - apply (IH s'); [ assumption | |].
     + now apply HA2 with s.
-  - split.
-    + intros u Hbeta; rewrite clos_rt_rt1n_iff in Hbeta;
-      inv Hbeta; [ assumption |]. inv H.
-      apply (IH s').
-      * assumption.
-      * now apply (HA2 s).
-      * now apply clos_rt_rt1n_iff.
-    + intros v Hbeta. rewrite clos_rt_rt1n_iff in Hbeta;
-        inv Hbeta. inv H.
-      apply (IH s').
-      * assumption.
-      * now apply (HA2 s).
-      * now apply clos_rt_rt1n_iff.
+    + now apply clos_rt_rt1n_iff.
+
+  - apply (IH s'); [ assumption | |].
+    + now apply HA2 with s.
+    + now apply clos_rt_rt1n_iff.
 Qed.
 
-Lemma reducible_sum2 (A B: type) (s: term):
+Lemma reducible_sum_injR (A B: type) (s: term):
   reducible B s ->
-  reducible (Sum A B) (In2 s).
+  reducible (Sum A B) (InjR s).
 Proof.
-  intros Hreds. simpl.
+  intros Hreds; simpl.
+
   specialize (reducible_is_SN B) as (HB1 & HB2 & HB3).
   assert (HSN: SN s) by now apply HB1.
-  induction HSN as [s _ IH]. split.
-  - apply Strong. intros t' Hstep. inv Hstep. apply IH.
-    + assumption.
+
+  induction HSN as [s _ IH].
+  split.
+  { apply Strong; intros t' Hstep.
+    inv Hstep.
+    apply IH; [ assumption |].
+    now apply HB2 with s. }
+
+  all: split.
+  all: intros ? Hbeta.
+  all: rewrite clos_rt_rt1n_iff in Hbeta.
+  all: inv Hbeta; try assumption.
+  all: inv H.
+
+  - apply (IH s'); [ assumption | |].
     + now apply HB2 with s.
-  - split.
-    + intros u Hbeta; rewrite clos_rt_rt1n_iff in Hbeta;
-      inv Hbeta. inv H.
-      apply (IH s').
-      * assumption.
-      * now apply (HB2 s).
-      * now apply clos_rt_rt1n_iff.
-    + intros v Hbeta. rewrite clos_rt_rt1n_iff in Hbeta;
-        inv Hbeta; [ assumption |]. inv H.
-      apply (IH s').
-      * assumption.
-      * now apply (HB2 s).
-      * now apply clos_rt_rt1n_iff.
+    + now apply clos_rt_rt1n_iff.
+
+  - apply (IH s'); [ assumption | |].
+    + now apply HB2 with s.
+    + now apply clos_rt_rt1n_iff.
 Qed.
 
 Lemma reducible_pat (A B C: type) (t u v: term):
   reducible (Sum A B) t ->
   reducible (Arr A C) (Lam u) ->
   reducible (Arr B C) (Lam v) ->
-  reducible C (Pat t u v).
+  reducible C (Case t u v).
 Proof.
   intros Hredt Hredu Hredv.
+
   specialize (reducible_is_SN (Arr A C)) as (HAC1 & HAC2 & HAC3).
   specialize (reducible_is_SN (Arr B C)) as (HBC1 & HBC2 & HBC3).
   specialize (reducible_is_SN (Sum A B)) as (H1 & H2 & H3).
   specialize (reducible_is_SN C) as (HC1 & HC2 & HC3).
 
   assert (HSNt: SN t) by now apply H1.
-  assert (HSNu: SN u). {
-    apply SN_sub_term with (Lam u).
-    - apply HAC1. assumption.
-    - apply Sub_lam.
-  }
+  assert (HSNu: SN u).
+  { apply SN_sub_term with (Lam u).
+    - now apply HAC1.
+    - apply Sub_Lam. }
 
-  assert (HSNv: SN v). {
-    apply SN_sub_term with (Lam v).
-    - apply HBC1. assumption.
-    - apply Sub_lam.
-  }
+  assert (HSNv: SN v).
+  { apply SN_sub_term with (Lam v).
+    - now apply HBC1.
+    - apply Sub_Lam. }
 
-  revert Hredt Hredu Hredv. apply SN_triple_ind with (t := t) (u := u) (v := v).
-  2, 3, 4: assumption.
-  intros t0 u0 v0 IH Hredt0 Hredu0 Hredv0. apply HC3; [ exact I |].
-  intros t' Hstep. inv Hstep.
-  - apply IH; try assumption.
-    + right. now right.
-    + apply H2 with t0; assumption.
-  - apply IH; try assumption.
-    + right. now left.
-    + apply HAC2 with (Lam u0); [ assumption | now apply Beta_Lam ].
-  - apply IH; try assumption.
+  revert Hredt Hredu Hredv.
+  apply SN_triple_ind with (t := t) (u := u) (v := v); [| assumption.. ].
+
+  intros t0 u0 v0 IH Hredt0 Hredu0 Hredv0.
+  apply HC3; [ exact I |].
+
+  intros t' Hstep.
+  inv Hstep.
+
+  - apply IH; [| | assumption.. ].
+    + now right; right.
+    + now apply H2 with t0.
+
+  - apply IH; [| assumption | | assumption ].
+    + now right; left.
+    + apply HAC2 with (Lam u0); [ assumption |].
+      now apply Beta_Lam.
+
+  - apply IH; [ | assumption..  |].
     + now left.
-    + apply HBC2 with (Lam v0); [ assumption | now apply Beta_Lam ].
-  - enough (reducible C (App (Lam u0) t1)).
-    + apply HC2 with (App (Lam u0) t1).
-      * assumption.
-      * now apply Beta_Subst.
-    + simpl in Hredu0. apply Hredu0. apply Hredt0. apply rt_refl.
-  - enough (reducible C (App (Lam v0) t1)).
-    + apply HC2 with (App (Lam v0) t1).
-      * assumption.
-      * now apply Beta_Subst.
-    + simpl in Hredv0. apply Hredv0. apply Hredt0. apply rt_refl.
+    + apply HBC2 with (Lam v0); [ assumption |].
+      now apply Beta_Lam.
+
+  - assert (reducible C (App (Lam u0) t1)).
+    { simpl in Hredu0.
+      apply Hredu0.
+      apply Hredt0.
+      apply rt_refl. }
+
+    apply HC2 with (App (Lam u0) t1); [ assumption |].
+    now apply Beta_Subst.
+
+  - assert (reducible C (App (Lam v0) t1)).
+    { simpl in Hredv0.
+      apply Hredv0.
+      apply Hredt0.
+      apply rt_refl. }
+
+    apply HC2 with (App (Lam v0) t1); [ assumption |].
+    now apply Beta_Subst.
 Qed.
 
 Lemma typing_is_reducible (Γ: var -> type) (σ: var -> term):
@@ -474,40 +508,48 @@ Lemma typing_is_reducible (Γ: var -> type) (σ: var -> term):
     forall (A: type) (t: term), Γ ⊢ t : A -> reducible A t.[σ].
 Proof.
   intros Hred A t.
-  revert Hred.
-  revert σ A Γ.
+  revert σ A Γ Hred.
 
   induction t; intros σ A Γ Hred.
   all: inversion 1; subst.
-
   - apply Hred.
+
   - apply IHt1 with (σ := σ) in H2; [| assumption ].
     apply IHt2 with (σ := σ) in H4; [| assumption ].
     now apply H2.
+
   - apply reducible_abs.
-    intros u Hredu. asimpl.
+    intros u Hredu; asimpl.
     apply IHt with (A0 .: Γ); [| assumption ].
     intros [| x ]; simpl; [ assumption |].
     apply Hred.
 
   - apply reducible_pair.
-    + now eapply IHt1.
-    + now eapply IHt2.
+    + now apply IHt1 with Γ.
+    + now apply IHt2 with Γ.
 
   - apply (IHt σ (Prod A B) Γ Hred H1).
   - apply (IHt σ (Prod A0 A) Γ Hred H1).
 
-  - simpl. apply reducible_pat with A0 B.
+  - simpl.
+    apply reducible_pat with A0 B.
     + now apply IHt with Γ.
-    + apply reducible_abs. intros u0 Hredu0.
-      asimpl. apply IHt0 with (A0 .: Γ); [| assumption ].
+    + apply reducible_abs.
+      intros; asimpl.
+      apply IHt0 with (A0 .: Γ); [| assumption ].
       intros [| x ]; simpl; [ assumption | apply Hred ].
-    + apply reducible_abs. intros. asimpl. apply IHt1 with (B .: Γ); [| assumption ].
+    + apply reducible_abs.
+      intros; asimpl.
+      apply IHt1 with (B .: Γ); [| assumption ].
       intros [| x ]; simpl; [ assumption | apply Hred ].
-  - change (reducible (Sum A0 B) (In1 t.[σ])).
-    apply reducible_sum1. now apply IHt with Γ.
-  - change (reducible (Sum A0 B) (In2 t.[σ])).
-    apply reducible_sum2. now apply IHt with Γ.
+
+  - replace ((InjL t).[σ]) with (InjL t.[σ]) by reflexivity.
+    apply reducible_sum_injL.
+    now apply IHt with Γ.
+
+  - replace ((InjR t).[σ]) with (InjR t.[σ]) by reflexivity.
+    apply reducible_sum_injR.
+    now apply IHt with Γ.
 Qed.
 
 Corollary STLC_is_SN (A: type) (Γ: var -> type) (t: term):
@@ -516,8 +558,10 @@ Proof.
   intros.
   apply (reducible_is_SN A).
   replace t with t.[ids] by apply subst_id.
+
   apply typing_is_reducible with Γ; [| assumption ].
   intros.
+
   apply reducible_var with Γ.
   now apply Typing_Var.
 Qed.
