theories/Base.v
@@ -1,3 +1,15 @@
 Require Export Nat.
+Require Export Relations.Relations.
 
 #[export] Set Default Goal Selector "!".
+
+Notation "R *" := (clos_refl_trans _ R)
+  (at level 8, no associativity, format "R *").
+
+Tactic Notation "inv" hyp(H) :=
+  inversion H; subst; clear H.
+
+Tactic Notation "inv" hyp(H) "as" simple_intropattern(pat) :=
+  let H' := fresh "H'" in
+  rename H into H';
+  inversion H' as pat; subst; clear H'.
