theories/SimplyTypedLambdaCalculus/Term.v
@@ -1,0 +1,209 @@
+From FormArith Require Export Base.
+
+From Autosubst Require Export Autosubst.
+
+
+Inductive term : Type :=
+  | Var (n: var)
+
+  (* Basic lambda calculus *)
+  | App (s t: term)
+  | Lam (s: {bind term})
+
+  (* Pairs and projections *)
+  | Pair (s t: term)
+  | ProjL (s: term)
+  | ProjR (s: term)
+
+  (* Injections and pattern matching *)
+  | Case (t: term) (u: {bind term}) (v: {bind term})
+  | InjL (s: term)
+  | InjR (s: term).
+
+(* Autosubst required magic *)
+Instance Ids_term: Ids term. derive. Defined.
+Instance Rename_term: Rename term. derive. Defined.
+Instance Subst_term: Subst term. derive. Defined.
+Instance SubstLemmas_term: SubstLemmas term. derive. Defined.
+
+
+Reserved Notation "t ~> t'" (at level 60).
+
+Inductive beta: term -> term -> Prop :=
+  (* Classical beta reduction *)
+  | Beta_Subst (s s' t: term): s' = s.[t .: ids] -> (App (Lam s) t) ~> s'
+  | Beta_AppL (s s' t: term): s ~> s' -> App s t ~> App s' t
+  | Beta_AppR (s t t': term): t ~> t' -> App s t ~> App s t'
+  | Beta_Lam (s s': term): s ~> s' -> Lam s ~> Lam s'
+
+  (* Pairs and projections *)
+  | Beta_Pair1 (s s' t: term): s ~> s' -> Pair s t ~> Pair s' t
+  | Beta_Pair2 (s t t': term): t ~> t' -> Pair s t ~> Pair s t'
+  | Beta_ProjL (s s': term): s ~> s' -> ProjL s ~> ProjL s'
+  | Beta_ProjR (s s': term): s ~> s' -> ProjR s ~> ProjR s'
+  | Beta_ProjL_Pair (s t: term): ProjL (Pair s t) ~> s
+  | Beta_ProjR_Pair (s t: term): ProjR (Pair s t) ~> t
+
+  (* Injections and pattern matching *)
+  | Beta_Case1 (t t' u v: term): t ~> t' -> Case t u v ~> Case t' u v
+  | Beta_Case2 (t u u' v: term): u ~> u' -> Case t u v ~> Case t u' v
+  | Beta_Case3 (t u v v': term): v ~> v' -> Case t u v ~> Case t u v'
+  | Beta_InjL (s s': term): s ~> s' -> InjL s ~> InjL s'
+  | Beta_InjR (s s': term): s ~> s' -> InjR s ~> InjR s'
+  | Beta_Case_InjL (t u u' v: term): u' = u.[t .: ids] -> Case (InjL t) u v ~> u'
+  | Beta_Case_InjR (t u v v': term): v' = v.[t .: ids] -> Case (InjR t) u v ~> v'
+
+  where "t ~> t'" := (beta t t').
+
+Notation "t ~>* t'" := (beta* t t') (at level 70, t' at next level).
+
+
+Lemma beta_subst (t t': term) (σ: var -> term):
+  t ~> t' -> t.[σ] ~> t'.[σ].
+Proof.
+  revert t' σ.
+
+  induction t as [
+    | ? IHs ? IHt | s IHs
+    | s IHs t IHt | s IHs | s IHs
+    | t IHt u IHu v IHv | s IHs | s IHs
+  ].
+
+  (* Classical lambda calculus *)
+  - intros ? ? Hbeta.
+    inv Hbeta.
+
+  - intros ? ? Hbeta.
+    inv Hbeta.
+    + apply Beta_Subst; asimpl.
+      reflexivity.
+
+    + apply Beta_AppL.
+      now apply IHs.
+
+    + apply Beta_AppR.
+      now apply IHt.
+
+  - intros ? ? Hbeta.
+    inv Hbeta.
+    apply Beta_Lam.
+    now apply IHs.
+
+  (* Pairs and projections *)
+  - intros ? ? Hbeta.
+    inv Hbeta.
+    + apply Beta_Pair1.
+      now apply IHs.
+    + apply Beta_Pair2.
+      now apply IHt.
+
+  - intros ? ? Hbeta.
+    inv Hbeta.
+    + apply Beta_ProjL.
+      now apply IHs.
+    + apply Beta_ProjL_Pair.
+
+  - intros ? ? Hbeta.
+    inv Hbeta.
+    + apply Beta_ProjR.
+      now apply IHs.
+    + apply Beta_ProjR_Pair.
+
+  (* Pattern matching and injections *)
+  - intros ? ? Hbeta.
+    inv Hbeta.
+    + apply Beta_Case1.
+      now apply IHt.
+    + apply Beta_Case2.
+      now apply IHu.
+    + apply Beta_Case3.
+      now apply IHv.
+
+    + apply Beta_Case_InjL; asimpl.
+      reflexivity.
+    + apply Beta_Case_InjR; asimpl.
+      reflexivity.
+
+  - intros ? ? Hbeta.
+    inv Hbeta.
+    apply Beta_InjL.
+    now apply IHs.
+
+  - intros ? ? Hbeta.
+    inv Hbeta.
+    apply Beta_InjR.
+    now apply IHs.
+Qed.
+
+
+Ltac apply_step Hred Hstep :=
+  induction Hstep; [
+    apply rt_step; now apply Hred |
+    apply rt_refl |
+    eapply rt_trans; eassumption
+  ].
+
+Lemma beta_star_context_unary (f: term -> term) (s s': term):
+  (forall (s s': term), s ~> s' -> f s ~> f s') ->
+  s ~>* s' -> f s ~>* f s'.
+Proof.
+  intros Hred Hstep.
+  apply_step Hred Hstep.
+Qed.
+
+Lemma beta_star_context_binary (f: term -> term -> term) (s s' t t': term):
+  (forall (s s' t: term), s ~> s' -> f s t ~> f s' t) ->
+  (forall (s t t': term), t ~> t' -> f s t ~> f s t') ->
+  s ~>* s' -> t ~>* t' -> f s t ~>* f s' t'.
+Proof.
+  intros Hred1 Hred2 Hstep1 Hstep2.
+
+  apply rt_trans with (f s' t).
+  { apply_step Hred1 Hstep1. }
+
+  apply_step Hred2 Hstep2.
+Qed.
+
+Lemma beta_star_context_ternary (f: term -> term -> term -> term) (s s' t t' u u': term):
+  (forall (s s' t u: term), s ~> s' -> f s t u ~> f s' t u) ->
+  (forall (s t t' u: term), t ~> t' -> f s t u ~> f s t' u) ->
+  (forall (s t u u': term), u ~> u' -> f s t u ~> f s t u') ->
+  s ~>* s' -> t ~>* t' -> u ~>* u' -> f s t u ~>* f s' t' u'.
+Proof.
+  intros Hred1 Hred2 Hred3 Hstep1 Hstep2 Hstep3.
+
+  apply rt_trans with (f s' t u).
+  { apply_step Hred1 Hstep1. }
+
+  apply rt_trans with (f s' t' u).
+  { apply_step Hred2 Hstep2. }
+
+  apply_step Hred3 Hstep3.
+Qed.
+
+Lemma beta_star_lam (s s': term):
+  s ~>* s' ->
+  Lam s ~>* Lam s'.
+Proof.
+  apply beta_star_context_unary.
+  apply Beta_Lam.
+Qed.
+
+Lemma beta_star_app (s s' t t': term):
+  s ~>* s' -> t ~>* t' ->
+  App s t ~>* App s' t'.
+Proof.
+  apply beta_star_context_binary.
+  - apply Beta_AppL.
+  - apply Beta_AppR.
+Qed.
+
+Lemma beta_star_case (s s' t t' u u': term):
+  s ~>* s' -> t ~>* t' -> u ~>* u' ->
+  Case s t u ~>* Case s' t' u'.
+Proof.
+  apply beta_star_context_ternary.
+  - apply Beta_Case1.
+  - apply Beta_Case2.
+  - apply Beta_Case3.
+Qed.
