theories/SimplyTypedLambdaCalculus/Typing.v
@@ -1,0 +1,253 @@
+From FormArith Require Export Base.
+From FormArith.SimplyTypedLambdaCalculus Require Import Term.
+
+
+Inductive type :=
+  | Base
+  | Arr (A B: type)
+  | Prod (A B: type)
+  | Sum (A B: type).
+
+
+Reserved Notation "Γ ⊢ t : A" (at level 60, t at next level).
+
+Inductive typing (Γ: var -> type): term -> type -> Prop :=
+  (* Classical lambda calculus *)
+  | Typing_Var (x: var) (A: type):
+      Γ x = A -> Γ ⊢ Var x : A
+
+  | Typing_App (s t: term) (A B: type) :
+      Γ ⊢ s : Arr A B ->
+      Γ ⊢ t : A ->
+      Γ ⊢ App s t : B
+
+  | Typing_Lam (s: term) (A B: type):
+      A .: Γ ⊢ s : B ->
+      Γ ⊢ Lam s : Arr A B
+
+  (* Pairs and projections *)
+  | Typing_ProjL (s: term) (A B: type):
+      Γ ⊢ s : Prod A B ->
+      Γ ⊢ ProjL s : A
+
+  | Typing_ProjR (s: term) (A B: type):
+      Γ ⊢ s : Prod A B ->
+      Γ ⊢ ProjR s : B
+
+  | Typing_Pair (s t: term) (A B: type):
+      Γ ⊢ s : A ->
+      Γ ⊢ t : B ->
+      Γ ⊢ Pair s t : Prod A B
+
+  (* Pattern matching and injections *)
+  | Typing_InjL (s: term) (A B: type):
+      Γ ⊢ s : A ->
+      Γ ⊢ InjL s : Sum A B
+
+  | Typing_InjR (s: term) (A B: type):
+      Γ ⊢ s : B ->
+      Γ ⊢ InjR s : Sum A B
+
+  | Typing_Sum (t u v: term) (A B C: type):
+      Γ ⊢ t : Sum A B ->
+      (A .: Γ) ⊢ u : C ->
+      (B .: Γ) ⊢ v : C ->
+      Γ ⊢ Case t u v : C
+  where "Γ ⊢ t : A" := (typing Γ t A).
+
+
+Lemma type_weakening (Γ: var -> type) (s: term) (A: type):
+  Γ ⊢ s : A ->
+    forall (Γ': var -> type) (x': var -> var),
+      Γ = x' >>> Γ' -> Γ' ⊢ s.[ren x'] : A.
+Proof.
+  induction 1 as [
+    ? ? ? H |
+    ? ? ? A ? _ IH1 _ IH2 |
+    ? ? A B _ IH |
+    ? ? A B _ IH |
+    ? ? ? ? _ IH |
+    ? ? ? ? ? _ IH1 _ IH2 |
+    ? ? A B _ IH |
+    ? ? A B _ IH  |
+    ? ? ? ? A B C _ IH1 _ IH2 _ IH3
+  ]; intros ? ? HΓ; simpl.
+
+  (* Classical lambda calculus *)
+  - apply Typing_Var.
+    now rewrite HΓ in H.
+
+  - apply Typing_App with A.
+    + now apply IH1.
+    + now apply IH2.
+
+  - apply Typing_Lam; asimpl.
+    apply IH.
+    now rewrite HΓ; asimpl.
+
+  (* Product types *)
+  - apply Typing_ProjL with B.
+    now apply IH.
+
+  - apply Typing_ProjR with A.
+    now apply IH.
+
+  - apply Typing_Pair.
+    + now apply IH1.
+    + now apply IH2.
+
+  (* Case types *)
+  - apply Typing_InjL.
+    now apply IH.
+
+  - apply Typing_InjR.
+    now apply IH.
+
+  - apply Typing_Sum with A B; asimpl.
+    + now apply IH1.
+    + apply IH2.
+      now rewrite HΓ; asimpl.
+    + apply IH3.
+      now rewrite HΓ; asimpl.
+Qed.
+
+Lemma type_subst (Γ Γ': var -> type) (s: term) (A: type) (σ: var -> term):
+  Γ ⊢ s : A ->
+  (forall (x: var), Γ' ⊢ σ x : Γ x) ->
+  Γ' ⊢ s.[σ] : A.
+Proof.
+  revert Γ Γ' A σ.
+
+  induction s as [
+    | ? IH1 ? IH2 | ? IH
+    | ? IH1 ? IH2 | ? IH | ? IH
+    | ? IH1 ? IH2 ? IH3 | ? IH | ? IH
+  ];
+  intros Γ Γ' ? ? HΓ HΓ'; simpl.
+
+  all: inv HΓ as [ | ? ? A' | ? A' | | | | | | ].
+
+  - apply HΓ'.
+
+  - apply Typing_App with A'.
+    + now apply IH1 with Γ.
+    + now apply IH2 with Γ.
+
+  - apply Typing_Lam.
+    apply IH with (A' .: Γ); [ assumption |].
+    intros [| x ]; asimpl.
+    + now apply Typing_Var.
+    + now apply type_weakening with Γ'.
+
+  - apply Typing_Pair.
+    + now apply IH1 with Γ.
+    + now apply IH2 with Γ.
+
+  - apply Typing_ProjL with B.
+    now apply IH with Γ.
+
+  - apply Typing_ProjR with A0.
+    now apply IH with Γ.
+
+  - apply Typing_Sum with (A := A0) (B := B).
+    + now apply IH1 with Γ.
+    + apply IH2 with (A0 .: Γ); [ assumption |].
+      intros [| x ]; asimpl.
+      * now apply Typing_Var.
+      * now apply type_weakening with Γ'.
+    + apply IH3 with (B .: Γ); [ assumption |].
+      intros [| x ]; asimpl.
+      * now apply Typing_Var.
+      * now apply type_weakening with Γ'.
+
+  - apply Typing_InjL.
+    now apply IH with Γ.
+
+  - apply Typing_InjR.
+    now apply IH with Γ.
+Qed.
+
+Lemma type_preservation (Γ: var -> type) (s t: term) (A: type):
+  Γ ⊢ s : A -> s ~> t -> Γ ⊢ t : A.
+Proof.
+  revert Γ t A.
+
+  induction s as [
+    | ? IH1 ? IH2 | ? IH
+    | ? IH1 ? IH2 | ? IH | ? IH
+    | ? IH1 ? IH2 ? IH3 | ? IH | ? IH
+  ]; intros Γ ? ? HΓ HΓ'; asimpl.
+
+  all: inv HΓ.
+  all: inv HΓ'.
+  
+  all: match goal with
+       | H: _ ⊢ _ : Arr ?A _ |- _ => rename A into A'
+       | H: _ ⊢ _ : Prod ?A _ |- _ => rename A into A'
+       | H: _ ⊢ _ : Case ?A _ |- _ => rename A into A'
+       | _ => idtac
+       end.
+
+  - match goal with
+    | H: Γ ⊢ Lam s : _ |- _ => inv H
+    end.
+
+    apply type_subst with (A' .: Γ); [ assumption |].
+    intros [| x ]; asimpl; [ assumption |].
+    now apply Typing_Var.
+
+  - apply Typing_App with A'; [| assumption ].
+    now apply IH1.
+
+  - apply Typing_App with A'; [ assumption |].
+    now apply IH2.
+
+  - apply Typing_Lam.
+    now apply IH.
+
+  - apply Typing_Pair.
+    + now apply IH1.
+    + assumption.
+
+  - apply Typing_Pair.
+    + assumption.
+    + now apply IH2.
+
+  - apply Typing_ProjL with B.
+    now apply IH.
+
+  - now inv H0.
+
+  - apply Typing_ProjR with A'.
+    now apply IH.
+
+  - now inv H0.
+
+  - apply Typing_Sum with A0 B.
+    2, 3: assumption.
+    now apply IH1.
+
+  - apply Typing_Sum with A0 B.
+    1, 3: assumption.
+    now apply IH2.
+
+  - apply Typing_Sum with A0 B.
+    1, 2: assumption.
+    now apply IH3.
+
+  - apply type_subst with (A0 .: Γ); [ assumption |].
+    intros [| x ]; asimpl.
+    + now inv H2.
+    + now apply Typing_Var.
+
+  - apply type_subst with (B .: Γ); [ assumption |].
+    intros [| x ]; asimpl.
+    + now inv H2.
+    + now apply Typing_Var.
+
+  - apply Typing_InjL.
+    now apply IH.
+
+  - apply Typing_InjR.
+    now apply IH.
+Qed.
